try migrate cmem

scratch/Scratch_Fib.thy
@@ -58,7 +58,6 @@ sepref_definition fib_rec1 is fib_rec :: "nat_assn\<^sup>k \<rightarrow>\<^sub>a
 
 definition fib_rec_mem_body :: "((int list \<times> nat) \<Rightarrow> (int list \<times> int) nres) \<Rightarrow> (int list \<times> nat) \<Rightarrow> (int list \<times> int) nres" where
   "fib_rec_mem_body \<equiv> \<lambda>f (t, n). do {
-    ASSERT (n < length t);
     tn \<leftarrow> mop_list_get t n;
     if tn \<ge> 0
       then RETURN (t, tn)
@@ -86,3 +85,32 @@ sepref_definition fib_rec_mem1 is fib_rec_mem :: "nat_assn\<^sup>k \<rightarrow>
   unfolding fib_rec_mem_def fib_rec_mem_body_def
   apply (rewrite in "RECT _ (\<hole>, _)" array_fold_custom_of_list)
   by sepref
+
+term 0 (**)
+
+definition cmem :: "int list \<Rightarrow> bool" where
+  "cmem M \<equiv> \<forall>i. i<length M \<longrightarrow> M!i\<ge>0 \<longrightarrow> M!i=fib i"
+
+lemma cmem_intro:
+  assumes "\<And>i. i<length M \<Longrightarrow> M!i\<ge>0 ==> M!i=fib i"
+  shows "cmem M"
+  using assms unfolding cmem_def by fastforce
+
+lemma cmem_elim:
+  assumes "cmem M" "i < length M"
+  obtains "M!i < 0" | "fib i = M!i "
+  using assms unfolding cmem_def by fastforce
+  term 0 
+
+lemma cmem_update:
+  "\<lbrakk>cmem M; v = fib i\<rbrakk> \<Longrightarrow> cmem (list_update M i v)"
+  by (fastforce intro!: cmem_intro elim: cmem_elim simp: nth_list_update')
+  
+
+
+
+
+
+
+
+
